misc PR comments, and move CMK + Grant Tokens to subtypes

src/KMS/KMSUtils.dfy
@@ -9,12 +9,32 @@ module {:extern "KMSUtils"} KMSUtils {
   import opened UInt = StandardLibrary.UInt
   import UTF8
 
-  const PROVIDER_ID := "aws-kms"
+  const MAX_GRANT_TOKENS := 10
 
-  function method ProviderID(): (id: UTF8.ValidUTF8Bytes)
-  {
-    UTF8.Encode(PROVIDER_ID).value
+  //FIXME: Figure out why this keeps timing out.
+  type CustomerMasterKey = s: string | ValidFormatCMK(s) witness "alias/ExampleAlias"
+  //type CustomerMasterKey = string
+
+  predicate method ValidFormatCMK(cmk: string) {
+    ValidFormatCMKKeyARN(cmk) || ValidFormatCMKAlias(cmk) || ValidFormatCMKAliasARN(cmk)
   }
+
+  predicate method ValidFormatCMKKeyARN(cmk: string) {
+    var components := Split(cmk, ':');
+    0 < |cmk| <= 2048 && |components| == 6 && components[0] == "arn" && components[2] == "kms" && Split(components[5], '/')[0] == "key"
+  }
+
+  predicate method ValidFormatCMKAlias(cmk: string) {
+    var components := Split(cmk, '/');
+    0 < |cmk| <= 2048 && |components| == 2 && components[0] == "alias"
+  }
+
+  predicate method ValidFormatCMKAliasARN(cmk: string) {
+    var components := Split(cmk, ':');
+    0 < |cmk| <= 2048 && |components| == 6 && components[0] == "arn" && components[2] == "kms" && Split(components[5], '/')[0] == "alias"
+  }
+
+  type GrantToken = s: string | 0 < |s| <= 8192 witness "witness"
 
   trait ClientSupplier {
     method GetClient(region: Option<string>) returns (res: Result<KMSClient>)
@@ -25,42 +45,55 @@ module {:extern "KMSUtils"} KMSUtils {
     method {:extern} GetClient(region: Option<string>) returns (res: Result<KMSClient>)
   }
 
-  datatype DataKeySpec = AES_128 | AES_256
-
-  datatype ResponseMetadata = ResponseMetadata(metadate: map<string, string>, requestID: string)
+  datatype ResponseMetadata = ResponseMetadata(metadata: map<string, string>, requestID: string)
 
   type HttpStatusCode = int //FIXME: Restrict this
 
-
-  datatype GenerateDataKeyRequest = GenerateDataKeyRequest(encryptionContext: Mat.EncryptionContext, grantTokens: seq<string>, keyID: string, numberOfBytes: int32)
+  datatype GenerateDataKeyRequest = GenerateDataKeyRequest(encryptionContext: Mat.EncryptionContext, grantTokens: seq<GrantToken>, keyID: CustomerMasterKey, numberOfBytes: int32)
+  {
+    predicate Valid() {
+      0 <= |grantTokens| <= MAX_GRANT_TOKENS && 0 < numberOfBytes <= 1024
+    }
+  }
 
   datatype GenerateDataKeyResponse = GenerateDataKeyResponse(ciphertextBlob: seq<uint8>, contentLength: int, httpStatusCode: HttpStatusCode, keyID: string, plaintext: seq<uint8>, responseMetadata: ResponseMetadata)
   {
     predicate method IsWellFormed() {
-      StringIs8Bit(keyID) && |keyID| < UINT16_LIMIT && |ciphertextBlob| < UINT16_LIMIT
+      |keyID| < UINT16_LIMIT && |ciphertextBlob| < UINT16_LIMIT
     }
   }
 
-
-  datatype EncryptRequest = EncryptRequest(encryptionContext: Mat.EncryptionContext, grantTokens: seq<string>, keyID: string, plaintext: seq<uint8>)
+  datatype EncryptRequest = EncryptRequest(encryptionContext: Mat.EncryptionContext, grantTokens: seq<GrantToken>, keyID: CustomerMasterKey, plaintext: seq<uint8>)
+  {
+    predicate Valid() {
+      0 <= |grantTokens| <= MAX_GRANT_TOKENS
+    }
+  }
 
   datatype EncryptResponse = EncryptResponse(ciphertextBlob: seq<uint8>, contentLength: int, httpStatusCode: HttpStatusCode, keyID: string, responseMetadata: ResponseMetadata)
   {
     predicate method IsWellFormed() {
-      StringIs8Bit(keyID) && |keyID| < UINT16_LIMIT && |ciphertextBlob| < UINT16_LIMIT
+      |keyID| < UINT16_LIMIT && |ciphertextBlob| < UINT16_LIMIT
     }
   }
 
-  datatype DecryptRequest = DecryptRequest(ciphertextBlob: seq<uint8>, encryptionContext: Mat.EncryptionContext, grantTokens: seq<string>)
+  datatype DecryptRequest = DecryptRequest(ciphertextBlob: seq<uint8>, encryptionContext: Mat.EncryptionContext, grantTokens: seq<GrantToken>)
+  {
+    predicate Valid() {
+      0 <= |grantTokens| <= MAX_GRANT_TOKENS
+    }
+  }
 
   datatype DecryptResponse = DecryptResponse(contentLength: int, httpStatusCode: HttpStatusCode, keyID: string, plaintext: seq<uint8>, responseMetadata: ResponseMetadata)
 
   // https://docs.aws.amazon.com/sdkfornet/v3/apidocs/items/KeyManagementService/TKeyManagementServiceClient.html
   class KMSClient {
     method {:extern} GenerateDataKey(request: GenerateDataKeyRequest) returns (res: Result<GenerateDataKeyResponse>)
+      requires request.Valid()
       //TODO mmtj: Should this be marked as modifying all of request's fields?
 
 	method {:extern} Encrypt(request: EncryptRequest) returns (res: Result<EncryptResponse>)
+      requires request.Valid()
       //TODO mmtj: Should this be marked as modifying all of request's fields?
 
     method {:extern} Decrypt(request: DecryptRequest) returns (res: Result<DecryptResponse>)
