src/Main.dfy
@@ -65,7 +65,8 @@ module Main {
       return;
     }
 
-    var generator := "arn:aws:kms:us-west-2:658956600833:key/b3537ef1-d8dc-4780-9f5a-55776cbb2f7f";
+    var generatorStr := "arn:aws:kms:us-west-2:658956600833:key/b3537ef1-d8dc-4780-9f5a-55776cbb2f7f";
+    var generator: KMSUtils.CustomerMasterKey := generatorStr;
     var clientSupplier := new KMSUtils.DefaultClientSupplier();
     var keyring := new KMSKeyring.KMSKeyring(clientSupplier, [], Some(generator), []);
     var cmm := new DefaultCMMDef.DefaultCMM.OfKeyring(keyring);
